cedar-lean/Cedar/Thm/Utils.lean
@@ -51,7 +51,7 @@ theorem mapM_over_map {α β γ} [Monad m] [LawfulMonad m] {f : α → β} {g : 
 theorem mapM_some_iff_f_some_on_all_elements {f : α → Option β} {list : List α} :
   Option.isSome (list.mapM f) ↔ ∀ x ∈ list, Option.isSome (f x)
 := by
-  rw [←List.mapM'_eq_mapM]
+  rw [← List.mapM'_eq_mapM]
   constructor
   case mp =>
     induction list
@@ -81,3 +81,49 @@ theorem mapM_some_iff_f_some_on_all_elements {f : α → Option β} {list : List
       have h₂ := h y ; simp at h₂
       rw [List.mapM'_cons]
       sorry
+
+/--
+  A generic lemma about the behavior of List.mapM' in the Except monad
+-/
+theorem mapM_ok_iff_f_ok_on_all_elements {f : α → Except ε β} {list : List α} :
+  Except.isOk (list.mapM f) ↔ ∀ x ∈ list, Except.isOk (f x)
+:= by
+  rw [← List.mapM'_eq_mapM]
+  simp [Except.isOk, Except.toBool]
+  constructor
+  case mp =>
+    induction list
+    case nil =>
+      intro _ x h₂
+      simp at h₂
+    case cons y ys h_ind =>
+      intro h₁ x h₂
+      unfold List.mapM' at h₁
+      cases h₄ : (f y) <;> simp [h₄] at h₁
+      case error => cases h₁
+      case ok b =>
+        rcases (List.mem_cons.mp h₂) with h₅ | h₅
+        case inl => rw [← h₅] at h₄; simp [h₄]
+        case inr =>
+          apply h_ind ; clear h_ind
+          case a =>
+            split at h₁ <;> split <;> simp
+            case h_1.h_2 h₅ _ _ h₆ =>
+              simp [h₆] at h₅
+              cases h₅
+            case h_2.h_2 => simp at h₁
+          case a => exact h₅
+  case mpr =>
+    induction list
+    case nil => simp [List.mapM', pure, Except.pure]
+    case cons x xs h_ind =>
+      intro h₂
+      split <;> simp
+      case h_2 err h₃ =>
+        cases h₄ : (f x) <;> simp [h₄] at h₂
+        case ok b =>
+          specialize h_ind h₂
+          split at h_ind <;> simp at h_ind
+          case h_1 err h₆ =>
+            simp [h₄, h₆, List.mapM', pure, Except.pure] at h₃
+            cases h₃
